lean/Lawean.lean
@@ -9,3 +9,5 @@ import Lawean.Sem
 import Lawean.SemTheorems
 import Lawean.SemExamples
 import Lawean.Properties
+import Lawean.Frame
+import Lawean.FrameExamples
